%!TEX root = /Users/sebi/Documents/uni/Master/Semester2/ML1Stuff/assignment1/main.tex
\section*{Probability Theory}

\begin{eqnarray} 
    p(x|z)p(y|x,z) &=&  \frac{p(x,z)}{p(z)}\cdot \frac{p(x,y,z)}{p(x,z)} \hspace{1cm}\mbox{2 times product rule}\\
    &=&  \frac{p(x,y,z)}{p(z)} \\
    &=&  p(x,y|z) \hspace{1cm} \mbox{Bayes Rule}
\end{eqnarray}

\begin{eqnarray}
    \frac{p(y| x,z)p(x|z)}{p(y|z)}&=& \frac{\frac{p(x,y,z)}{p(x,z)} \frac{p(x,z)}{p(z)}}{\frac{p(y,z)}{p(z)}} \hspace{1cm}\mbox{3 times Bayes Rule}\\
    &=& \frac{p(x,y,z)}{p(y,z)} \\
    &=& p(x|y,z) \hspace{1cm}\mbox{Bayes Rule}
\end{eqnarray}


\begin{eqnarray}
    \mathbb{E}[X]+\mathbb{E}[Y]&=& \sum_{X}(x_i p(x_i)) + \sum_{Y}(y_i p(y_i))\\
    &=& \sum_{X, Y}(x_i p(x_i)p(y_i)) + \sum_{X,Y}(y_i p(x_i)p(y_i))\\
    &=& \sum_{X, Y}(x_i p(x_i,y_i)) + \sum_{X,Y}(y_i p(x_i,y_i)) \hspace{4mm}\mbox{because of independence}\\
    &=& \sum_{X, Y}((x_i+y_i) p(x_i,y_i))\hspace{1cm}\\
    &=& \mathbb{E}[X+Y]
\end{eqnarray}

\begin{eqnarray}
    \text{var}[X+Y]&=& \mathbb{E}[(X+Y)^2] - [\mathbb{E}[X+Y]]^2\\
    &=& \mathbb{E}[X^2+2XY+Y^2] - [\mathbb{E}[X]+\mathbb{E}[Y]]^2 \hspace{5mm}\mbox{using (3)}\\
    &=& \mathbb{E}[X^2]+\mathbb{E}[2XY]+\mathbb{E}[Y^2] - [\mathbb{E}[X]+\mathbb{E}[Y]]^2 \hspace{5mm}\mbox{using (3)}\\
    &=& \mathbb{E}[X^2]+\mathbb{E}[2XY]+\mathbb{E}[Y^2] - \mathbb{E}[X]^2-2[\mathbb{E}[X]\mathbb{E}[Y]] -\mathbb{E}[Y]^2 \\
    &=& \mathbb{E}[X^2]- \mathbb{E}[X]^2 +\mathbb{E}[Y^2]-\mathbb{E}[Y]^2 -2[\mathbb{E}[X]\mathbb{E}[Y]] +\mathbb{E}[2XY]  \\
    &=& \text{var}[X] +\text{var}[Y] -2[\mathbb{E}[X]\mathbb{E}[Y]] +\mathbb{E}[XY]]  \\
    &=& \text{var}[X] +\text{var}[Y] -2[\text{covar}[X,Y]]  \\
    &=& \text{var}[X] +\text{var}[Y]\hspace{5mm}\mbox{since X,Y are uncorrelated} 
\end{eqnarray}
