%!TEX root = main.tex
\section*{Feature Transformation - 1} 

\begin{align}
	\phi \Bigg( \begin{matrix}
		x_1 \\ x_2
	\end{matrix} \Bigg) &= \begin{pmatrix}
		x_1^3 \\ \sqrt{3} x_1^2 x_2 \\ \sqrt{3} x_1 x_2^2 \\ x_2^3
	\end{pmatrix} \\
	\langle \phi(x), \phi(x') \rangle &= \begin{pmatrix}
		x_1^3 \\ \sqrt{3} x_1^2 x_2 \\ \sqrt{3} x_1 x_2^2 \\ x_2^3
	\end{pmatrix}^\top
 	\begin{pmatrix}
			{x'}_{1}^{3} \\ \sqrt{3} {x'}_1^2 x'_2 \\ \sqrt{3} {x'}_1 {x'}_2^2 \\ {x'}_2^3
	\end{pmatrix}\\
		&= x_1^3 {x'}_1^3 + 3x_1^2 {x'}_1^2 x_2 {x'}_2 + 3x_1 {x'}_1 x_2^2 {x'}_2^2 + x_2^3 {x'}_2^3\\
		&= (x_1 {x'}_1 + x_2 {x'}_2)^3
\end{align}



\begin{eqnarray}
    k(x,x')&=&\left(<x,x'> + c \right)^3 \\
    &=&\left(x_1x_1'+x_2x_2'+ c \right)^3 \\
    &=&(x_1x_1')^3 + 3(x_1x_1')(x_2x_2')^2 + 3(x_1x_1')c^2 + 3(x_1x_1')^2(x_2x_2')  \\ \nonumber
    && + 3(x_1x_1')^2c  + 6(x_1x_1')(x_2x_2')c + (x_2x_2')^3 + 3 (x_2x_2')c^2 + 3 c (x_2x_2')^2 + c^3\\
    &=& (x_1x_1')((x_1x_1')((x_1x_1') + 3((x_2x_2') + c)) + (3x_2x_2')((x_2x_2') + 2c) + 3c^2)  \\ \nonumber
    && (x_2x_2')((x_2x_2')((x_2x_2') + 3 c)+ 3c^2) + c^3
\end{eqnarray}