%!TEX root=main.tex

\section*{Structured Output Prediction} 
We want to derive the dual programm of
\begin{align}
	&\min_w \frac{1}{2} \sum_{c=1}^C ||w_c||^2\\
	&sb.t. \langle w, \phi(x_i,y_i)\rangle - \langle w, \phi(x_i,y)\rangle \geq 1 , \forall i=1,...,N, y=1,...,C,y \neq y_i \notag
\end{align}
We first write down the Lagrangian
\begin{align}
	\mathcal{L}(w,\alpha) &=
	\frac{1}{2} \sum_{c=1}^C ||w_c||^2 - 
	\sum_{i=1}^N \sum_{\begin{subarray}{l} y=1 \\ y\neq y_i \end{subarray}}^C
	\alpha_{i,y}(\langle w, \phi(x_i,y_i)\rangle - \langle w, \phi(x_i,y)\rangle - 1 ) \\
	sb.t. ~ &\alpha_{i,y} \geq 0 ~ \forall i = 1,...,N ~ \forall y = 1,...,C ~ ,~ y\neq y_i\notag \\
	&= \frac{1}{2} \sum_{c=1}^C ||w_c||^2 - \sum_{i=1}^N \sum_{\begin{subarray}{l} y=1 \\ y\neq y_i \end{subarray}}^C \alpha_{i,y}(\langle w_{y_i}, \phi(x_i)\rangle - \langle w_y, \phi(x_i)\rangle - 1 ) 
\end{align}
And take the derivatives wrt. $w_{y_i}$ and $w_y$
\begin{align}
	\frac{\partial \mathcal{L}}{\partial w_{y_i}} &= w_{y_i} - 
	\sum_{i=1}^N \sum_{\begin{subarray}{l} y=1 \\ y\neq y_i \end{subarray}}^C
	\alpha_{i,y} \phi(x_i) \stackrel{!}{=} 0 \\
	w_{y_i} &= \sum_{i=1}^N \sum_{\begin{subarray}{l} y=1 \\ y\neq y_i \end{subarray}}^C
	\alpha_{i,y} \phi(x_i) \\
	\frac{\partial \mathcal{L}}{\partial w_{y}} &= w_{y} + 
	\sum_{i=1}^N 
	\alpha_{i,y} \phi(x_i) \stackrel{!}{=} 0 \\
	w_{y} &= - \sum_{i=1}^N \alpha_{i,y} \phi(x_i)
\end{align}
We can now substitiute $w$ in the Lagrangian
\begin{align}
	\mathcal{L}(w,\alpha) &= 
	\frac{1}{2} \sum_{c=1}^C ||w_c||^2 
	 - \sum_{i=1}^N \sum_{\begin{subarray}{l} y=1 \\ y\neq y_i \end{subarray}}^C 
	   \alpha_{i,y} \langle w_{y_i}, \phi(x_i)\rangle 
	 + \sum_{i=1}^N \sum_{\begin{subarray}{l} y=1 \\ y\neq y_i \end{subarray}}^C 
	   \alpha_{i,y} \langle w_y, \phi(x_i)\rangle 
	 + \sum_{i=1}^N \sum_{\begin{subarray}{l} y=1 \\ y\neq y_i \end{subarray}}^C 
	 	\alpha_{i,y} \\
	&=  \frac{1}{2} \sum_{c=1}^C ||w_c||^2 
	 - \sum_{i=1}^N \sum_{\begin{subarray}{l} y=1 \\ y\neq y_i \end{subarray}}^C 
		\sum_{j=1}^N \sum_{\begin{subarray}{l} z=1 \\ z\neq z_j \end{subarray}}^C 
	   \alpha_{i,y} \alpha_{j,z} \phi(x_i) \phi(x_j) 
	 - \sum_{i=1}^N \sum_{\begin{subarray}{l} y=1 \\ y\neq y_i \end{subarray}}^C 
	\sum_{j=1}^N 
	   \alpha_{i,y} \alpha_{j,y} \phi(x_i) \phi(x_j) 
	 + \sum_{i=1}^N \sum_{\begin{subarray}{l} y=1 \\ y\neq y_i \end{subarray}}^C 
	 	\alpha_{i,y}
\end{align}
\begin{align}
	\frac{1}{2} \sum_{y=1}^C ||w_y||^2 &= 
	\frac{1}{2}(||w_{y_i}||^2 + \sum_{\begin{subarray}{l} y=1 \\ y\neq y_i \end{subarray}}^C || w_y ||^2)\\
	&= \frac{1}{2}\left( \sum_{i=1}^N \sum_{\begin{subarray}{l} y=1 \\ y\neq y_i \end{subarray}}^C 
		\sum_{j=1}^N \sum_{\begin{subarray}{l} z=1 \\ z\neq z_j \end{subarray}}^C 
	   \alpha_{i,y} \alpha_{j,z} \phi(x_i) \phi(x_j) 
	 +\sum_{i=1}^N \sum_{\begin{subarray}{l} y=1 \\ y\neq y_i \end{subarray}}^C 
	\sum_{j=1}^N 
	   \alpha_{i,y} \alpha_{j,y} \phi(x_i) \phi(x_j) 
	  \right) 
\end{align}
\begin{align}
	\mathcal{L}(\alpha) &= \sum_{i=1}^N \sum_{\begin{subarray}{l} y=1 \\ y\neq y_i \end{subarray}}^C \alpha_{i,y} -\frac{1}{2}\left( \sum_{i=1}^N \sum_{\begin{subarray}{l} y=1 \\ y\neq y_i \end{subarray}}^C 
		\sum_{j=1}^N \sum_{\begin{subarray}{l} z=1 \\ z\neq z_j \end{subarray}}^C 
	   \alpha_{i,y} \alpha_{j,z} \phi(x_i) \phi(x_j) 
	 +\sum_{i=1}^N \sum_{\begin{subarray}{l} y=1 \\ y\neq y_i \end{subarray}}^C 
	\sum_{j=1}^N 
	   \alpha_{i,y} \alpha_{j,y} \phi(x_i) \phi(x_j) 
	  \right)\\
	&sb.t. ~ \alpha_{i,y} \geq 0 ~ \forall i = 1,...,N ~ \forall y = 1,...,C ~ ,~ y\neq y_i\notag
\end{align}
In the kernelized version we get
\begin{align}
	\mathcal{L}(\alpha) &= \sum_{i=1}^N \sum_{\begin{subarray}{l} y=1 \\ y\neq y_i \end{subarray}}^C \alpha_{i,y} -\frac{1}{2}\left( \sum_{i=1}^N \sum_{\begin{subarray}{l} y=1 \\ y\neq y_i \end{subarray}}^C 
		\sum_{j=1}^N \sum_{\begin{subarray}{l} z=1 \\ z\neq z_j \end{subarray}}^C 
	   \alpha_{i,y} \alpha_{j,z} k(x_i,x_j)
	 +\sum_{i=1}^N \sum_{\begin{subarray}{l} y=1 \\ y\neq y_i \end{subarray}}^C 
	\sum_{j=1}^N 
	   \alpha_{i,y} \alpha_{j,y} k(x_i,x_j) 
	  \right)\\
	sb.t. ~ &\alpha_{i,y} \geq 0 ~ \forall i = 1,...,N ~ \forall y = 1,...,C ~ ,~ y\neq y_i\notag
\end{align}
For the soft-margin case we have similar results
\begin{align} 
	\mathcal{L}(w,\alpha, \beta) &=
	\frac{1}{2} \sum_{c=1}^C ||w_c||^2 + \mathcal{C}\sum_{i=1}^N \xi_i - 
	\sum_{i=1}^N \sum_{\begin{subarray}{l} y=1 \\ y\neq y_i \end{subarray}}^C
	\alpha_{i,y}(\langle w, \phi(x_i,y_i)\rangle - \langle w, \phi(x_i,y)\rangle - 1 +\xi_i )
	- \sum_{i}^N  \beta_i \xi_i \\
	sb.t. ~ &\alpha_{i,y} \geq 0 ~, ~\beta_i \geq 0 ~ \forall i = 1,...,N ~ \forall y = 1,...,C ~ ,~ y\neq y_i\notag
\end{align}
\begin{align}
	\frac{\partial \mathcal{L}}{\partial \xi_i} &= \mathcal{C} - \sum_{\begin{subarray}{l} y=1 \\ y\neq y_i \end{subarray}}^C \alpha_{i,y} - \beta_i \stackrel{!}{=} 0 \\
	\sum_{\begin{subarray}{l} y=1 \\ y\neq y_i \end{subarray}}^C \alpha_{i,y} &= \mathcal{C} -\beta_i
\end{align}
\begin{align}
	\mathcal{L}(\alpha) &= \sum_{i=1}^N \sum_{\begin{subarray}{l} y=1 \\ y\neq y_i \end{subarray}}^C \alpha_{i,y} -\frac{1}{2}\left( \sum_{i=1}^N \sum_{\begin{subarray}{l} y=1 \\ y\neq y_i \end{subarray}}^C 
		\sum_{j=1}^N \sum_{\begin{subarray}{l} z=1 \\ z\neq z_j \end{subarray}}^C 
	   \alpha_{i,y} \alpha_{j,z} k(x_i,x_j)
	 +\sum_{i=1}^N \sum_{\begin{subarray}{l} y=1 \\ y\neq y_i \end{subarray}}^C 
	\sum_{j=1}^N 
	   \alpha_{i,y} \alpha_{j,y} k(x_i,x_j) 
	  \right)\\
   sb.t. ~ &\alpha_{i,y} \geq 0 ~ \forall i = 1,...,N ~ \forall y = 1,...,C ~ ,~ y\neq y_i\notag \\
	&\mathcal{C} \geq \sum_{\begin{subarray}{l} y=1 \\ y\neq y_i \end{subarray}}^C \alpha_{i,y} \notag
\end{align}

