%!TEX root = ./main.tex
\section*{Matrix Derivatives}


\begin{eqnarray}
    \frac{\partial}{\partial x}w^Tx&=& \frac{\partial}{\partial x} \sum_{i=1}^N w_i x_i  \\
    &=&\left(\frac{\partial}{\partial x_1}, \dots, \frac{\partial}{\partial x_n} \right) \sum_{i=1}^N w_i x_i \\
    &=&\left(\frac{\partial}{\partial x_1}\sum_{i=1}^N w_i x_i , \dots, \frac{\partial}{\partial x_n} \sum_{i=1}^N w_i x_i \right) \\
    &=& (w_1,\dots,w_n) = w
\end{eqnarray}


Ich glaub das hier ist noch mist:

\begin{eqnarray}
    \frac{\partial}{\partial x}x^TAx&=& \frac{\partial}{\partial x} x^T \left( \sum_{i=1}^n A_{i,1} x_i,\dots,\sum_{i=1}^n A_{i,n} x_i \right) \\
    &=& \frac{\partial}{\partial x} \left( \begin{matrix} 
    \sum_{i=1}^n A_{i,1} x_i x_1 & \dots &\sum_{i=1}^n A_{i,n} x_i x_1 \\
    \vdots&&\vdots \\
    \sum_{i=1}^n A_{i,1} x_i x_n & \dots &\sum_{i=1}^n A_{i,n} x_i x_n \\
    \end{matrix}\right)
\end{eqnarray}